\section{Problems}

\begin{Pb}
Falling object.\\

An object of mass $m$ is falling with velocity $v$. We take into account the force exerted by gravity $-mg$, and the air drag $-\alpha v$. 
\begin{enumerate}
\item Apply the FPD to find the equation satisfied by $v$: \[v' = g-\frac{\alpha}{m}v.\]
\item Solve the equation.
\end{enumerate}
\end{Pb}

\begin{Pb}
Solve the following nonhomogeneous linear differential equations.
\begin{enumerate}
\item $y' + y = \sin(t)$,
\item $y' + 4y = \tan(2t)$, \\
\ \\
\textbf{Hint:} \[\int \frac{dt}{cos(2t)} = \int\frac{du}{1-u^2}\]
where we use the half-angle parametrization $u = \tan (t/2) $.
\item $(1+t^2 ) y' = ty + (1+t^2)$,
\item $(t+1) y' + ty = (t+1)^2$.
\end{enumerate}
\end{Pb}

\begin{Pb} 
Solve the following differential equations. Recall that we saw their meaning and their derivation in class.
\begin{enumerate}
\item Free fall with air drag
\[v' + \frac{\alpha}{m} v = g,\]
\item Linearized pendulum equation
\[\theta'' + \frac{g}{L}\theta = 0\]
\item Logistic equation for growth model in population dynamics
\[P' = r(1-\frac{P}{K}) P. \]
\item Spring mass equation
\[x'' + \frac{k}{m}x = k L_0\]
\item Oscillation with friction
\[x'' +\alpha x'+ \frac{k}{m}x = 0 \]
\end{enumerate}
\end{Pb}

\newpage
\begin{Pb}
Solve the following linear differential systems.
\begin{enumerate}
\item \[\left\{\begin{split}
x' & = 3x +y-z\\
y' & = 2y + z\\
z' & = 2z\\
\end{split}\right.\]
\item \[Y' = \begin{pmatrix} 1 & 2 \\ -1 & 4 \end{pmatrix} Y + \begin{pmatrix}2 \\ t\end{pmatrix}\]
\item \[\left\{\begin{split}
x' & = 2tx -y +t \cos t \\
y' & = x + 2ty + t \sin t\\
\end{split}\right.\]
Hint: for the homogeneous solution, the change of variable 
\[\left\{\begin{split}
u & = xe^{t^2} \\
v & = ye^{t^2} \\
\end{split}\right.\]
can be useful.
\item \[Y' = \begin{pmatrix} 4 & 2 \\ -1 & 1 \end{pmatrix} Y + \begin{pmatrix} \sin t \\ \cos t\end{pmatrix}\]
\end{enumerate} 
\end{Pb}

\begin{Pb}
Convert the following linear differential equations into first a order system of linear differential equations. 
\begin{enumerate}
\item $y'' + 3 y' +2y =0$
\item $y''' +4y'' -y' -4y =0 $
\item $y'' - y' -2y = \sin (t)$
\item Convert the following system of linear differential equations into a first order one
\[\left\{\begin{split}
x'' & = x+y \\
y'' & = x+ x' + y + y' \\
\end{split}\right.\]
\end{enumerate}
\end{Pb}

